Checkpoint

SSMorph.v
@@ -6,14 +6,89 @@ Require Import Fin.
 Require Import Interval.
 Require Import Lib.
 Require Import ScanState.
-Require Import FunctionalExtensionality.
+Require Import Hask.IEndo.
+Require Import Hask.IApplicative.
+Require Import Hask.IMonad.
+Require Import Hask.IState.
 
 Generalizable All Variables.
 
+Open Scope nat_scope.
 Open Scope program_scope.
 
 Module MSSMorph (M : Machine).
 Include MScanState M.
+
+Record SSInfo (H : ScanStateDesc -> Prop) (P : relation ScanStateDesc) := {
+    startDesc  : ScanStateDesc;
+    startHolds : H startDesc;
+    thisDesc   : ScanStateDesc;
+    thisHolds  : P startDesc thisDesc;
+    thisState  : ScanState thisDesc
+}.
+
+Arguments startDesc {H P} _.
+Arguments thisDesc  {H P} _.
+Arguments thisHolds {H P} _.
+Arguments thisState {H P} _.
+
+Definition SState (J K : ScanStateDesc -> Prop) (P Q : relation ScanStateDesc) :=
+  IState (SSInfo J P) (SSInfo K Q).
+
+(* Definition withCursor {P Q a} `{PreOrder _ P} *)
+(*   (f : forall sd : ScanStateDesc, ScanStateCursor sd -> SState P Q a) : SState P Q a := *)
+(*   rgets (fun s => exist _ (thisDesc s) (thisCursor s)) *)
+(*     >>= uncurry_sig f. *)
+
+Definition withScanState {J K P Q a}
+  (f : forall sd : ScanStateDesc, ScanState sd -> SState J K P Q a)
+  : SState J K P Q a :=
+  iget >>>= fun i => f (thisDesc i) (thisState i).
+
+(** Given an non-monadic function that returns a [NextScanState], absorb it
+    into the indexed monad appropriately. *)
+
+(*
+Definition step {H P} `{Transitive _ P} `(st : ScanState sd)
+  (n : NextScanState (P sd)) : SState H H P P unit.
+Proof.
+  constructor. intros i.
+  split. apply tt.
+  destruct i.
+  destruct n.
+  subst.
+  rapply Build_SSInfo.
+  apply startHolds0.
+  transitivity thisDesc0.
+    assumption.
+  apply morphProof0.
+  assumption.
+Defined.
+*)
+
+(* Arguments cursor {P a} f. *)
+Arguments withScanState {J K P Q a} f.
+(* Arguments step {H P _} f. *)
+
+Definition stbind {P Q R a b}
+  (f : (a -> IState Q R b)) (x : IState P Q a) : IState P R b :=
+  @ijoin IState _ P Q R b (@imap _ _ P Q _ _ f x).
+
+Notation "m >>>= f" := (stbind f m) (at level 25, left associativity).
+
+(* Notation "x <- c1 ;; c2" := (@ibind _ _ _ _ _ c1 (fun x => c2)) *)
+(*   (at level 100, c1 at next level, right associativity). *)
+
+Notation "X <<- A ; B" := (A >>>= (fun X => B))
+  (right associativity, at level 84, A1 at next level).
+
+(* Notation "x : a <== c1 ;; c2" := (@ibind _ _ _ _ _ c1 (fun x : a => c2)) *)
+(*   (at level 100, c1 at next level, right associativity). *)
+
+Notation "A ;;; B" := (_ <<- A ; B)
+  (right associativity, at level 84, A1 at next level).
+
+Definition return_ {I X} := @ipure IState _ I X.
 
 (** ** SSMorph *)
 
@@ -42,7 +117,7 @@ Obligation 2.
   transitivity (length (handled y)); auto.
 Qed.
 
-Record SSMorphSt (sd1 sd2 : ScanStateDesc) : Prop := {
+Record > SSMorphSt (sd1 sd2 : ScanStateDesc) : Prop := {
     st_is_SSMorph :> SSMorph sd1 sd2;
 
     total_extent_measurably_decreases :
@@ -72,9 +147,6 @@ Record SSMorphLen (sd1 sd2 : ScanStateDesc) : Prop := {
       length (unhandled sd1) > 0 -> length (unhandled sd2) > 0
 }.
 
-Definition newSSMorphLen (s : ScanStateDesc) : SSMorphLen s s.
-Proof. intros. constructor; auto. constructor; auto. Defined.
-
 Program Instance SSMorphLen_Trans : Transitive SSMorphLen.
 Obligation 1.
   constructor.
@@ -84,7 +156,17 @@ Obligation 1.
   intros. auto.
 Qed.
 
-Record SSMorphStLen (sd1 sd2 : ScanStateDesc) : Prop := {
+Program Instance SSMorphLen_PO : PreOrder SSMorphLen.
+Obligation 1.
+  unfold Reflexive. intros.
+  constructor. reflexivity.
+  intuition.
+Qed.
+
+Definition newSSMorphLen (s : ScanStateDesc) : SSMorphLen s s.
+Proof. intros. constructor; auto. constructor; auto. Defined.
+
+Record > SSMorphStLen (sd1 sd2 : ScanStateDesc) : Prop := {
     stlen_is_SSMorphLen :> SSMorphLen sd1 sd2;
     stlen_is_SSMorphSt  :> SSMorphSt sd1 sd2
 }.
@@ -225,6 +307,159 @@ Definition cursorFromMorphStLen `(cur : ScanStateCursor sd)
   `(n : NextState cur SSMorphStLen) : ScanStateCursor (nextDesc n) :=
   cursorFromMorphLen cur (NSS_transport _ _ n (stlen_is_SSMorphLen _ _)).
 
+Definition HasUnhandled := fun sd => length (unhandled sd) > 0.
+Definition MaybeHasUnhandled := fun sd => length (unhandled sd) >= 0.
+
+Definition withLenCursor {H Q a}
+  (f : forall sd : ScanStateDesc, ScanStateCursor sd
+         -> SState HasUnhandled H SSMorphLen Q a)
+  : SState HasUnhandled H SSMorphLen Q a.
+Proof.
+  constructor. intros i.
+  destruct i.
+  unfold HasUnhandled in startHolds0.
+  destruct thisHolds0.
+  pose proof startHolds0.
+  apply unhandled_nonempty0 in H0.
+  pose {| curState  := thisState0
+        ; curExists := H0 |} as p.
+  specialize (f thisDesc0 p).
+  destruct f as [res].
+  apply res.
+  rapply Build_SSInfo.
+  apply startHolds0.
+  rapply Build_SSMorphLen; auto.
+  apply len_is_SSMorph0.
+  apply thisState0.
+Defined.
+
+Definition weakenStLenToSt {H} : SState H H SSMorphStLen SSMorphSt unit.
+Proof.
+  constructor. intros HS.
+  split. constructor.
+  destruct HS.
+  rapply Build_SSInfo.
+  - apply startHolds0.
+  - destruct thisHolds0.
+    apply stlen_is_SSMorphSt0.
+  - assumption.
+Defined.
+
+(*
+Definition withStLenCursor {Q a}
+  (f : forall sd : ScanStateDesc, ScanStateCursor sd
+         -> SState HasUnhandled SSMorphStLen Q a)
+  : SState HasUnhandled SSMorphStLen Q a.
+Proof.
+  constructor. intros i.
+  destruct i.
+  pose (@withLenCursor Q a).
+  unfold HasUnhandled in startHolds0.
+  destruct thisHolds0.
+  pose proof startHolds0.
+  apply unhandled_nonempty0 in H.
+  pose {| curState  := thisState0
+        ; curExists := H |} as p.
+  specialize (f thisDesc0 p).
+  destruct f as [res].
+  apply res.
+  rapply Build_SSInfo.
+  apply startHolds0.
+  rapply Build_SSMorphLen; auto.
+  apply len_is_SSMorph0.
+  apply thisState0.
+Defined.
+*)
+
+(*
+Definition weakenStLenToSt H : SState SSMorphStLen SSMorphSt unit.
+Proof.
+  constructor. intros.
+  split. constructor.
+  destruct H.
+  rapply @Build_SState'.
+    destruct bridgeState0.
+    destruct morphProof0.
+    rapply Build_NextScanState.
+    apply nextState0.
+    apply stlen_is_SSMorphSt0.
+  destruct resultState0.
+  destruct morphProof0.
+  rapply Build_NextScanState.
+  apply nextState0.
+  apply stlen_is_SSMorphSt0.
+  Grab Existential Variables.
+  apply thisCursor0.
+  apply startCursor0.
+Defined.
+*)
+
+(*
+Definition weakenStLenToLen : SState SSMorphStLen SSMorphLen unit.
+Proof.
+  constructor. intros.
+  split. constructor.
+  destruct H as [sd s].
+  destruct s as [cur n].
+  unfold SState'.
+  exists sd.
+  exists cur.
+  destruct n.
+  eexists.
+  apply nextState0.
+  destruct morphProof0.
+  apply stlen_is_SSMorphLen0.
+Defined.
+*)
+
+Definition weakenStLenToLen {H} : SState H H SSMorphStLen SSMorphLen unit.
+Proof.
+  constructor. intros HS.
+  split. apply tt.
+  destruct HS.
+  rapply Build_SSInfo.
+  - apply startHolds0.
+  - destruct thisHolds0.
+    apply stlen_is_SSMorphLen0.
+  - assumption.
+Defined.
+
+Definition weakenHasUnhandled {P}
+  : SState HasUnhandled MaybeHasUnhandled P P unit.
+Proof.
+  constructor. intros HS.
+  split. apply tt.
+  destruct HS.
+  rapply Build_SSInfo.
+  - unfold HasUnhandled in startHolds0.
+    unfold MaybeHasUnhandled. omega.
+  - apply thisHolds0.
+  - assumption.
+Defined.
+
+(*
+Definition weakenStLenToLen : SState SSMorphStLen SSMorphLen unit.
+Proof.
+  constructor. intros.
+  split. constructor.
+  destruct H.
+  rapply @Build_SState'.
+    destruct bridgeState0.
+    destruct morphProof0.
+    rapply Build_NextScanState.
+    apply nextState0.
+    apply stlen_is_SSMorphLen0.
+  destruct resultState0.
+  destruct morphProof0.
+  rapply Build_NextScanState.
+  apply nextState0.
+  apply stlen_is_SSMorphLen0.
+  Grab Existential Variables.
+  apply thisCursor0.
+  apply startCursor0.
+Defined.
+*)
+
 (*
 Lemma ScanState_unhandledExtent_nonzero `(st : ScanState sd) :
   length (unhandled sd) > 0 <-> unhandledExtent sd > 0.
@@ -266,16 +501,83 @@ Proof.
 Qed.
 *)
 
-Definition moveUnhandledToActive `(cur : ScanStateCursor sd) (reg : PhysReg)
-  : NextState cur SSMorphSt.
+Definition moveUnhandledToActive (reg : PhysReg)
+  : SState HasUnhandled MaybeHasUnhandled SSMorphLen SSMorphSt unit.
 Proof.
-  destruct cur. destruct sd.
-  destruct unhandled0; simpl in *. omega.
+Admitted.
+(*
+  constructor. intros.
+  split. constructor.
+  destruct H.
+  destruct resultState0.
+  destruct morphProof0.
+  destruct nextDesc0.
+  destruct unhandled0; simpl in *.
+    destruct thisCursor0. omega.
   pose (ScanState_moveUnhandledToActive nextInterval0 unhandled0
           (* unhsort *)
           active0 inactive0 handled0 intervals0 assignments0
           fixedIntervals0 i reg lists_are_unique0).
-  eexists. apply s. apply curState0.
+  eapply {| startDesc   := startDesc0
+          ; startCursor := startCursor0
+          ; thisDesc    :=
+            {| nextInterval     := nextInterval0
+             ; unhandled        := i :: unhandled0
+             ; active           := active0
+             ; inactive         := inactive0
+             ; handled          := handled0
+             ; intervals        := intervals0
+             ; assignments      := assignments0
+             ; fixedIntervals   := fixedIntervals0
+             ; lists_are_unique := lists_are_unique0
+             |}
+          ; resultState := {| nextState := s nextState0 |}
+          |}.
+  Grab Existential Variables.
+  pose (NoDup_unhandledExtent_cons nextInterval0 i unhandled0 intervals0
+         (V.replace assignments0 i (Some reg)) assignments0 fixedIntervals0
+         (i :: active0) active0 inactive0 inactive0 handled0 handled0
+         (move_unhandled_to_active _ i unhandled0 active0 inactive0 handled0
+            lists_are_unique0) lists_are_unique0)
+      as ue_cons.
+  - rapply Build_SSMorphSt; auto.
+    rapply Build_SSMorph; auto.
+    intuition.
+  - admit.
+  - admit.
+Defined.
+*)
+
+(*
+Definition moveUnhandledToActive (reg : PhysReg)
+  : SState SSMorphLen SSMorphSt unit.
+Proof.
+  constructor. intros.
+  split. constructor.
+  destruct H as [sd p].
+  destruct p as [cur n].
+  destruct n.
+  destruct morphProof0.
+  destruct nextDesc0.
+  destruct unhandled0; simpl in *.
+    destruct cur. omega.
+  pose (ScanState_moveUnhandledToActive nextInterval0 unhandled0
+          (* unhsort *)
+          active0 inactive0 handled0 intervals0 assignments0
+          fixedIntervals0 i reg lists_are_unique0).
+  unfold SState'.
+  eexists         {|
+        nextInterval := nextInterval0;
+        unhandled := i :: unhandled0;
+        active := active0;
+        inactive := inactive0;
+        handled := handled0;
+        intervals := intervals0;
+        assignments := assignments0;
+        fixedIntervals := fixedIntervals0;
+        lists_are_unique := lists_are_unique0 |}.
+  eexists.
+  eexists. apply (s nextState0).
   pose (NoDup_unhandledExtent_cons nextInterval0 i unhandled0 intervals0
          (V.replace assignments0 i (Some reg)) assignments0 fixedIntervals0
          (i :: active0) active0 inactive0 inactive0 handled0 handled0
@@ -284,7 +586,26 @@ Proof.
     as ue_cons.
   rapply Build_SSMorphSt; auto.
   rapply Build_SSMorph; auto.
-  apply (Lt.lt_le_weak _ _ ue_cons).
+  intuition.
+  Grab Existential Variables.
+  rapply Build_ScanStateCursor.
+    apply nextState0.
+  simpl in *.
+  intuition.
+Defined.
+*)
+
+Definition moveActiveToHandled {H} `(x : IntervalId sd)
+  : SState (fun sd' => sd = sd' /\ In x (active sd)) H SSMorphLen SSMorphLen unit.
+Proof.
+  constructor. intros i.
+  split. apply tt.
+  destruct i.
+  intuition.
+  pose (ScanState_moveActiveToInactive thisDesc0 x thisState0 H1). eexists. apply s.
+  destruct sd. simpl.
+  rapply Build_SSMorphLen; auto.
+  rapply Build_SSMorph; auto.
 Defined.
 
 Definition moveActiveToHandled `(st : ScanState sd) (x : IntervalId sd)
